ChoicePrelude/StoreKeyAction.v
@@ -1,0 +1,144 @@
+(** * Generic stores: key actions *)
+
+From ChoicePrelude Require Export StoreCore.
+
+Section AbstractStoreKeyAction.
+
+Context {V : Type} `{ValueSig V}.
+
+Lemma storeA_swap_lookup {K : Type} `{Countable K} `{!SwapKey K}
+    (x y : K) (s : StoreA K) (z : K) :
+  ((storeA_swap x y s : gmap K V) !! key_swap x y z) =
+  ((s : gmap K V) !! z).
+Proof.
+  unfold storeA_swap.
+  change (kmap (M2:=gmap K) (key_swap x y) s !! key_swap x y z = s !! z).
+  pose proof (key_swap_inj x y) as Hinj.
+  rewrite (lookup_kmap (M1:=gmap K) (M2:=gmap K)
+    (Inj0:=Hinj) (key_swap x y) s z).
+  reflexivity.
+Qed.
+
+Lemma storeA_swap_lookup_inv {K : Type} `{Countable K} `{!SwapKey K}
+    (x y : K) (s : StoreA K) (z : K) :
+  ((storeA_swap x y s : gmap K V) !! z) =
+  ((s : gmap K V) !! key_swap x y z).
+Proof.
+  rewrite <- (key_swap_involutive x y z) at 1.
+  apply storeA_swap_lookup.
+Qed.
+
+Lemma storeA_swap_dom {K : Type} `{Countable K} `{!SwapKey K}
+    (x y : K) (s : StoreA K) :
+  dom (@storeA_swap V K _ _ _ x y s) = gset_swap x y (dom s).
+Proof.
+  unfold storeA_swap, gset_swap.
+  change (dom (kmap (M2:=gmap K) (key_swap x y) s) =
+    set_map (key_swap x y) (dom s)).
+  pose proof (key_swap_inj x y) as Hinj.
+  rewrite (dom_kmap_L (M:=gmap K) (M2:=gmap K)
+    (Inj0:=Hinj) (key_swap x y) s).
+  reflexivity.
+Qed.
+
+Lemma storeA_swap_delete {K : Type} `{Countable K} `{!SwapKey K}
+    (x y z : K) (s : StoreA K) :
+  storeA_swap x y (delete z s) =
+  delete (key_swap x y z) (storeA_swap x y s : gmap K V).
+Proof.
+  unfold storeA_swap.
+  change (kmap (M2:=gmap K) (key_swap x y) (delete z (s : gmap K V)) =
+    delete (key_swap x y z)
+      (kmap (M2:=gmap K) (key_swap x y) (s : gmap K V))).
+  refine (@kmap_delete K (gmap K) _ _ _ _ _ _ _ _ _
+    K (gmap K) _ _ _ _ _ _ _ _ _
+    (key_swap x y) _ V (s : gmap K V) z).
+  apply key_swap_inj.
+Qed.
+
+Lemma storeA_swap_insert {K : Type} `{Countable K} `{!SwapKey K}
+    (x y z : K) (v : V) (s : StoreA K) :
+  storeA_swap x y (<[z := v]> s) =
+  <[key_swap x y z := v]> (storeA_swap x y s : gmap K V).
+Proof.
+  unfold storeA_swap.
+  change (kmap (key_swap x y) (<[z := v]> (s : gmap K V)) =
+    (<[key_swap x y z := v]>
+      (kmap (key_swap x y) (s : gmap K V)) : gmap K V)).
+  refine (@kmap_insert K (gmap K) _ _ _ _ _ _ _ _ _
+    K (gmap K) _ _ _ _ _ _ _ _ _
+    (key_swap x y) _ V (s : gmap K V) z v).
+  apply key_swap_inj.
+Qed.
+
+Lemma storeA_swap_union {K : Type} `{Countable K} `{!SwapKey K}
+    (x y : K) (s1 s2 : StoreA K) :
+  storeA_swap x y (@union (gmap K V) _ s1 s2) =
+  @union (gmap K V) _ (storeA_swap x y s1 : gmap K V) (storeA_swap x y s2 : gmap K V).
+Proof.
+  unfold storeA_swap.
+  change (kmap (key_swap x y) (@union (gmap K V) _ (s1 : gmap K V) (s2 : gmap K V)) =
+    @union (gmap K V) _
+      (kmap (key_swap x y) (s1 : gmap K V))
+      (kmap (key_swap x y) (s2 : gmap K V))).
+  refine (@kmap_union K (gmap K) _ _ _ _ _ _ _ _ _
+    K (gmap K) _ _ _ _ _ _ _ _ _
+    (key_swap x y) _ V (s1 : gmap K V) (s2 : gmap K V)).
+  apply key_swap_inj.
+Qed.
+
+Lemma storeA_shift_lookup {K : Type} `{Countable K} `{!ShiftKey K}
+    (k : nat) (s : StoreA K) (z : K) :
+  ((storeA_shift k s : gmap K V) !! key_shift k z) =
+  ((s : gmap K V) !! z).
+Proof.
+  unfold storeA_shift.
+  rewrite (lookup_kmap (M1:=gmap K) (M2:=gmap K)
+    (Inj0:=key_shift_inj k) (key_shift k) s z).
+  reflexivity.
+Qed.
+
+Lemma storeA_shift_dom {K : Type} `{Countable K} `{!ShiftKey K}
+    (k : nat) (s : StoreA K) :
+  dom (@storeA_shift V K _ _ _ k s) = set_map (key_shift k) (dom s).
+Proof.
+  unfold storeA_shift.
+  change (dom (kmap (M2:=gmap K) (key_shift k) (s : gmap K V)) =
+    set_map (key_shift k) (dom (s : gmap K V))).
+  rewrite (dom_kmap_L (M:=gmap K) (M2:=gmap K)
+    (Inj0:=key_shift_inj k) (key_shift k) (s : gmap K V)).
+  reflexivity.
+Qed.
+
+Lemma storeA_shift_empty {K : Type} `{Countable K} `{!ShiftKey K} k :
+  storeA_shift k (∅ : StoreA K) = (∅ : gmap K V).
+Proof.
+  unfold storeA_shift.
+  change (kmap (M2:=gmap K) (key_shift k) (∅ : gmap K V) =
+    (∅ : gmap K V)).
+  apply kmap_empty.
+Qed.
+
+Lemma storeA_shift_insert {K : Type} `{Countable K} `{!ShiftKey K}
+    k z v (s : StoreA K) :
+  storeA_shift k (<[z := v]> s) =
+  <[key_shift k z := v]> (storeA_shift k s : gmap K V).
+Proof.
+  unfold storeA_shift.
+  rewrite (kmap_insert (M1:=gmap K) (M2:=gmap K)
+    (key_shift k) (Inj0:=key_shift_inj k) (A:=V) s z v).
+  reflexivity.
+Qed.
+
+Lemma storeA_shift_union {K : Type} `{Countable K} `{!ShiftKey K}
+    k (s1 s2 : StoreA K) :
+  storeA_shift k (@union (gmap K V) _ (s1 : gmap K V) (s2 : gmap K V)) =
+  (storeA_shift k s1 : gmap K V) ∪ (storeA_shift k s2 : gmap K V).
+Proof.
+  unfold storeA_shift.
+  rewrite (kmap_union (M1:=gmap K) (M2:=gmap K)
+    (key_shift k) (Inj0:=key_shift_inj k) (A:=V) s1 s2).
+  reflexivity.
+Qed.
+
+End AbstractStoreKeyAction.
